dataset/problems/003_dutch_national_flag/tests.dfy
@@ -1,60 +1,48 @@
-// Dutch National Flag -- Test cases
+// Dutch National Flag -- Runtime spec tests
+// Note: The spec predicates (AllValidColors, IsSortedColors) use array reads,
+// which can't be tested purely as predicates on sequences.
+// We test ValidColor (the core predicate) and seq-based equivalents.
 
 predicate ValidColor(c: int)
 {
   c == 0 || c == 1 || c == 2
 }
 
-predicate AllValidColors(a: array<int>)
-  reads a
+predicate AllValidColorsSeq(a: seq<int>)
 {
-  forall i :: 0 <= i < a.Length ==> ValidColor(a[i])
+  forall i | 0 <= i < |a| :: ValidColor(a[i])
 }
 
-predicate IsSortedColors(a: array<int>)
-  reads a
+predicate IsSortedColorsSeq(a: seq<int>)
 {
-  forall i, j :: 0 <= i < j < a.Length ==> a[i] <= a[j]
+  forall i, j | 0 <= i < j < |a| :: a[i] <= a[j]
 }
 
-method {:axiom} DutchFlag(a: array<int>)
-  requires AllValidColors(a)
-  modifies a
-  ensures IsSortedColors(a)
-  ensures AllValidColors(a)
-  ensures multiset(a[..]) == old(multiset(a[..]))
-
-method TestMixed()
+method Main()
 {
-  var a := new int[] [2, 0, 1, 2, 0, 1];
-  DutchFlag(a);
-  assert IsSortedColors(a);
-}
+  // Test ValidColor
+  expect ValidColor(0), "0 is a valid color";
+  expect ValidColor(1), "1 is a valid color";
+  expect ValidColor(2), "2 is a valid color";
+  expect !ValidColor(3), "3 is not a valid color";
+  expect !ValidColor(-1), "-1 is not a valid color";
+  expect !ValidColor(10), "10 is not a valid color";
 
-method TestAllSame()
-{
-  var a := new int[] [1, 1, 1];
-  DutchFlag(a);
-  assert IsSortedColors(a);
-}
+  // Test AllValidColorsSeq
+  expect AllValidColorsSeq([0, 1, 2, 0, 1, 2]), "all 0,1,2 should be valid";
+  expect AllValidColorsSeq([0, 0, 0]), "all zeros valid";
+  expect AllValidColorsSeq([]), "empty should be valid";
+  expect !AllValidColorsSeq([0, 1, 3]), "contains 3, not valid";
+  expect !AllValidColorsSeq([0, -1, 2]), "contains -1, not valid";
 
-method TestAlreadySorted()
-{
-  var a := new int[] [0, 0, 1, 2, 2];
-  DutchFlag(a);
-  assert IsSortedColors(a);
-}
+  // Test IsSortedColorsSeq
+  expect IsSortedColorsSeq([0, 0, 1, 1, 2, 2]), "sorted colors should be sorted";
+  expect IsSortedColorsSeq([0, 1, 2]), "0,1,2 sorted";
+  expect IsSortedColorsSeq([]), "empty sorted";
+  expect IsSortedColorsSeq([1]), "single sorted";
+  expect !IsSortedColorsSeq([2, 1, 0]), "reversed not sorted";
+  expect !IsSortedColorsSeq([1, 0, 2]), "1,0,2 not sorted";
+  expect IsSortedColorsSeq([0, 0, 0, 1, 2, 2]), "valid Dutch flag output";
 
-method TestReversed()
-{
-  var a := new int[] [2, 1, 0];
-  DutchFlag(a);
-  assert IsSortedColors(a);
-}
-
-method TestEmpty()
-{
-  var a := new int[] [];
-  DutchFlag(a);
-  assert IsSortedColors(a);
+  print "All spec tests passed\n";
 }
